codelib/CodeLib/SepLogic/SmallStepLifting.lean
@@ -3831,7 +3831,9 @@ theorem wp_load8U
     exact ⟨[],
       .running ⟨⟨params, localValues, .i32 byte.toUInt32 :: values⟩,
         code, arity, remainder, controls, calls⟩,
-      store, [], ⟨rfl, _, rfl, by simpa [Hread] using Step.load8U hbound⟩⟩
+      store, [], ⟨rfl, _, rfl,
+        by simpa [Hread] using
+          Step.load8U (α := α) (address := Value.i32 address) rfl hbound⟩⟩
   iintro !> %e₂ %store₂ %forks %Hstep Hcredit
   rcases Hstep with ⟨hforks, kind, hobs, wasmStep⟩
   change forks = [] at hforks
@@ -3843,7 +3845,8 @@ theorem wp_load8U
       (.instruction (.load8U offset))
       ⟨.running ⟨⟨params, localValues, .i32 byte.toUInt32 :: values⟩,
         code, arity, remainder, controls, calls⟩, store⟩ := by
-    simpa [Hread] using (Step.load8U (α := α) hbound)
+    simpa [Hread] using
+      (Step.load8U (α := α) (address := Value.i32 address) rfl hbound)
   obtain ⟨rfl, hconfig⟩ := step_deterministic expectedStep wasmStep
   have parts := Config.mk.inj hconfig
   have hexpr := parts.1
@@ -3983,7 +3986,7 @@ theorem wp_load8S
         code, arity, remainder, controls, calls⟩,
       store, [], ⟨rfl, _, rfl, by
         rw [show byte = store.wasm.mem.read8 (address + offset) from Hread.symm]
-        exact Step.load8S hbound⟩⟩
+        exact Step.load8S (address := Value.i32 address) rfl hbound⟩⟩
   iintro !> %e₂ %store₂ %forks %Hstep Hcredit
   rcases Hstep with ⟨hforks, kind, hobs, wasmStep⟩
   change forks = [] at hforks
@@ -3997,7 +4000,7 @@ theorem wp_load8S
         .i32 (Int32.ofInt (signExtend (byte.toUInt32.toNat % 256) 8)).toUInt32 :: values⟩,
         code, arity, remainder, controls, calls⟩, store⟩ := by
     rw [show byte = store.wasm.mem.read8 (address + offset) from Hread.symm]
-    exact Step.load8S (α := α) hbound
+    exact Step.load8S (α := α) (address := Value.i32 address) rfl hbound
   obtain ⟨rfl, hconfig⟩ := step_deterministic expectedStep wasmStep
   have parts := Config.mk.inj hconfig
   have hexpr := parts.1
@@ -4056,7 +4059,9 @@ theorem wp_load16U
     exact ⟨[],
       .running ⟨⟨params, localValues, .i32 (word &&& 0xFFFF) :: values⟩,
         code, arity, remainder, controls, calls⟩,
-      store, [], ⟨rfl, _, rfl, by simpa [Hread] using Step.load16U hbound⟩⟩
+      store, [], ⟨rfl, _, rfl,
+        by simpa [Hread] using
+          Step.load16U (α := α) (address := Value.i32 address) rfl hbound⟩⟩
   iintro !> %e₂ %store₂ %forks %Hstep Hcredit
   rcases Hstep with ⟨hforks, kind, hobs, wasmStep⟩
   change forks = [] at hforks
@@ -4068,7 +4073,8 @@ theorem wp_load16U
       (.instruction (.load16U offset))
       ⟨.running ⟨⟨params, localValues, .i32 (word &&& 0xFFFF) :: values⟩,
         code, arity, remainder, controls, calls⟩, store⟩ := by
-    simpa [Hread] using (Step.load16U (α := α) hbound)
+    simpa [Hread] using
+      (Step.load16U (α := α) (address := Value.i32 address) rfl hbound)
   obtain ⟨rfl, hconfig⟩ := step_deterministic expectedStep wasmStep
   have parts := Config.mk.inj hconfig
   have hexpr := parts.1
@@ -4133,7 +4139,7 @@ theorem wp_load16S
         code, arity, remainder, controls, calls⟩,
       store, [], ⟨rfl, _, rfl, by
         rw [show word &&& 0xFFFF = store.wasm.mem.read16 (address + offset) from Hread.symm]
-        exact Step.load16S hbound⟩⟩
+        exact Step.load16S (address := Value.i32 address) rfl hbound⟩⟩
   iintro !> %e₂ %store₂ %forks %Hstep Hcredit
   rcases Hstep with ⟨hforks, kind, hobs, wasmStep⟩
   change forks = [] at hforks
@@ -4147,7 +4153,7 @@ theorem wp_load16S
         .i32 (Int32.ofInt (signExtend ((word &&& 0xFFFF).toNat % 65536) 16)).toUInt32 :: values⟩,
         code, arity, remainder, controls, calls⟩, store⟩ := by
     rw [show word &&& 0xFFFF = store.wasm.mem.read16 (address + offset) from Hread.symm]
-    exact Step.load16S (α := α) hbound
+    exact Step.load16S (α := α) (address := Value.i32 address) rfl hbound
   obtain ⟨rfl, hconfig⟩ := step_deterministic expectedStep wasmStep
   have parts := Config.mk.inj hconfig
   have hexpr := parts.1
@@ -4598,7 +4604,8 @@ theorem wp_store8
       { store with wasm :=
           { store.wasm with
             mem := store.wasm.mem.write8 (address + offset) value.toUInt8 } },
-      [], ⟨rfl, _, rfl, Step.store8 hbound⟩⟩
+      [], ⟨rfl, _, rfl,
+        Step.store8 (α := α) (address := Value.i32 address) rfl hbound⟩⟩
   iintro !> %e₂ %store₂ %forks %Hstep Hcredit
   rcases Hstep with ⟨hforks, kind, hobs, wasmStep⟩
   change forks = [] at hforks
@@ -4614,7 +4621,7 @@ theorem wp_store8
             { store.wasm with
               mem := store.wasm.mem.write8
                 (address + offset) value.toUInt8 } }⟩ :=
-    Step.store8 hbound
+    Step.store8 (α := α) (address := Value.i32 address) rfl hbound
   obtain ⟨rfl, hconfig⟩ := step_deterministic expectedStep wasmStep
   have parts := Config.mk.inj hconfig
   have hexpr := parts.1
@@ -4758,7 +4765,8 @@ theorem wp_store16
       { store with wasm :=
           { store.wasm with
             mem := store.wasm.mem.write16 (address + offset) value } },
-      [], ⟨rfl, _, rfl, Step.store16 hbound⟩⟩
+      [], ⟨rfl, _, rfl,
+        Step.store16 (α := α) (address := Value.i32 address) rfl hbound⟩⟩
   iintro !> %e₂ %store₂ %forks %Hstep Hcredit
   rcases Hstep with ⟨hforks, kind, hobs, wasmStep⟩
   change forks = [] at hforks
@@ -4775,7 +4783,7 @@ theorem wp_store16
         { store with wasm :=
             { store.wasm with
               mem := store.wasm.mem.write16 (address + offset) value } }⟩ :=
-    Step.store16 hbound
+    Step.store16 (α := α) (address := Value.i32 address) rfl hbound
   obtain ⟨rfl, hconfig⟩ := step_deterministic expectedStep wasmStep
   have parts := Config.mk.inj hconfig
   have hexpr := parts.1
@@ -5006,7 +5014,9 @@ theorem wp_load32
     exact ⟨[],
       .running ⟨⟨params, localValues, .i32 word :: values⟩,
         code, arity, remainder, controls, calls⟩,
-      store, [], ⟨rfl, _, rfl, by simpa [Hread] using Step.load32 hbound⟩⟩
+      store, [], ⟨rfl, _, rfl,
+        by simpa [Hread] using
+          Step.load32 (α := α) (address := Value.i32 address) rfl hbound⟩⟩
   iintro !> %e₂ %store₂ %forks %Hstep Hcredit
   rcases Hstep with ⟨hforks, kind, hobs, wasmStep⟩
   change forks = [] at hforks
@@ -5018,7 +5028,8 @@ theorem wp_load32
       (.instruction (.load32 offset))
       ⟨.running ⟨⟨params, localValues, .i32 word :: values⟩,
         code, arity, remainder, controls, calls⟩, store⟩ := by
-    simpa [Hread] using (Step.load32 (α := α) hbound)
+    simpa [Hread] using
+      (Step.load32 (α := α) (address := Value.i32 address) rfl hbound)
   obtain ⟨rfl, hconfig⟩ := step_deterministic expectedStep wasmStep
   have parts := Config.mk.inj hconfig
   have hexpr := parts.1
@@ -5081,7 +5092,8 @@ theorem wp_store32
       { store with wasm :=
           { store.wasm with
             mem := store.wasm.mem.write32 (address + offset) value } },
-      [], ⟨rfl, _, rfl, Step.store32 hbound⟩⟩
+      [], ⟨rfl, _, rfl,
+        Step.store32 (α := α) (address := Value.i32 address) rfl hbound⟩⟩
   iintro !> %e₂ %store₂ %forks %Hstep Hcredit
   rcases Hstep with ⟨hforks, kind, hobs, wasmStep⟩
   change forks = [] at hforks
@@ -5098,7 +5110,7 @@ theorem wp_store32
         { store with wasm :=
             { store.wasm with
               mem := store.wasm.mem.write32 (address + offset) value } }⟩ :=
-    Step.store32 hbound
+    Step.store32 (α := α) (address := Value.i32 address) rfl hbound
   obtain ⟨rfl, hconfig⟩ := step_deterministic expectedStep wasmStep
   have parts := Config.mk.inj hconfig
   have hexpr := parts.1
@@ -9655,7 +9667,9 @@ theorem wp_load8UMemory64
     exact ⟨[],
       .running ⟨⟨params, localValues, .i32 byte.toUInt32 :: values⟩,
         code, arity, remainder, controls, calls⟩,
-      store, [], ⟨rfl, _, rfl, by simpa [Hread] using Step.load8UMemory64 hbound⟩⟩
+      store, [], ⟨rfl, _, rfl,
+        by simpa [Hread] using
+          Step.load8U (α := α) (address := Value.i64 address) rfl hbound⟩⟩
   iintro !> %e₂ %store₂ %forks %Hstep Hcredit
   rcases Hstep with ⟨hforks, kind, hobs, wasmStep⟩
   change forks = [] at hforks
@@ -9667,7 +9681,8 @@ theorem wp_load8UMemory64
       (.instruction (.load8U offset))
       ⟨.running ⟨⟨params, localValues, .i32 byte.toUInt32 :: values⟩,
         code, arity, remainder, controls, calls⟩, store⟩ := by
-    simpa [Hread] using (Step.load8UMemory64 (α := α) hbound)
+    simpa [Hread] using
+      (Step.load8U (α := α) (address := Value.i64 address) rfl hbound)
   obtain ⟨rfl, hconfig⟩ := step_deterministic expectedStep wasmStep
   have parts := Config.mk.inj hconfig
   have hexpr := parts.1
@@ -9729,7 +9744,7 @@ theorem wp_load8SMemory64
         code, arity, remainder, controls, calls⟩,
       store, [], ⟨rfl, _, rfl, by
         rw [show byte = store.wasm.mem.read8 (address.toUInt32 + offset) from Hread.symm]
-        exact Step.load8SMemory64 hbound⟩⟩
+        exact Step.load8S (address := Value.i64 address) rfl hbound⟩⟩
   iintro !> %e₂ %store₂ %forks %Hstep Hcredit
   rcases Hstep with ⟨hforks, kind, hobs, wasmStep⟩
   change forks = [] at hforks
@@ -9743,7 +9758,7 @@ theorem wp_load8SMemory64
         .i32 (Int32.ofInt (signExtend (byte.toUInt32.toNat % 256) 8)).toUInt32 :: values⟩,
         code, arity, remainder, controls, calls⟩, store⟩ := by
     rw [show byte = store.wasm.mem.read8 (address.toUInt32 + offset) from Hread.symm]
-    exact Step.load8SMemory64 hbound
+    exact Step.load8S (address := Value.i64 address) rfl hbound
   obtain ⟨rfl, hconfig⟩ := step_deterministic expectedStep wasmStep
   have parts := Config.mk.inj hconfig
   have hexpr := parts.1
@@ -9802,7 +9817,9 @@ theorem wp_load16UMemory64
     exact ⟨[],
       .running ⟨⟨params, localValues, .i32 (word &&& 0xFFFF) :: values⟩,
         code, arity, remainder, controls, calls⟩,
-      store, [], ⟨rfl, _, rfl, by simpa [Hread] using Step.load16UMemory64 hbound⟩⟩
+      store, [], ⟨rfl, _, rfl,
+        by simpa [Hread] using
+          Step.load16U (α := α) (address := Value.i64 address) rfl hbound⟩⟩
   iintro !> %e₂ %store₂ %forks %Hstep Hcredit
   rcases Hstep with ⟨hforks, kind, hobs, wasmStep⟩
   change forks = [] at hforks
@@ -9814,7 +9831,8 @@ theorem wp_load16UMemory64
       (.instruction (.load16U offset))
       ⟨.running ⟨⟨params, localValues, .i32 (word &&& 0xFFFF) :: values⟩,
         code, arity, remainder, controls, calls⟩, store⟩ := by
-    simpa [Hread] using Step.load16UMemory64 hbound
+    simpa [Hread] using
+      Step.load16U (α := α) (address := Value.i64 address) rfl hbound
   obtain ⟨rfl, hconfig⟩ := step_deterministic expectedStep wasmStep
   have parts := Config.mk.inj hconfig
   have hexpr := parts.1
@@ -9878,7 +9896,7 @@ theorem wp_load16SMemory64
       store, [], ⟨rfl, _, rfl, by
         rw [show word &&& 0xFFFF = store.wasm.mem.read16 (address.toUInt32 + offset)
             from Hread.symm]
-        exact Step.load16SMemory64 hbound⟩⟩
+        exact Step.load16S (address := Value.i64 address) rfl hbound⟩⟩
   iintro !> %e₂ %store₂ %forks %Hstep Hcredit
   rcases Hstep with ⟨hforks, kind, hobs, wasmStep⟩
   change forks = [] at hforks
@@ -9893,7 +9911,7 @@ theorem wp_load16SMemory64
         code, arity, remainder, controls, calls⟩, store⟩ := by
     rw [show word &&& 0xFFFF = store.wasm.mem.read16 (address.toUInt32 + offset)
         from Hread.symm]
-    exact Step.load16SMemory64 hbound
+    exact Step.load16S (address := Value.i64 address) rfl hbound
   obtain ⟨rfl, hconfig⟩ := step_deterministic expectedStep wasmStep
   have parts := Config.mk.inj hconfig
   have hexpr := parts.1
@@ -9952,7 +9970,8 @@ theorem wp_store8Memory64
           { store.wasm with
             mem := store.wasm.mem.write8 (address.toUInt32 + offset) value.toUInt8 } },
       [], ⟨rfl, _, rfl,
-        by simpa only [Wasm.SmallStep.setMemory_eq] using Step.store8Memory64 hbound⟩⟩
+        by simpa only [Wasm.SmallStep.setMemory_eq] using
+          Step.store8 (α := α) (address := Value.i64 address) rfl hbound⟩⟩
   iintro !> %e₂ %store₂ %forks %Hstep Hcredit
   rcases Hstep with ⟨hforks, kind, hobs, wasmStep⟩
   change forks = [] at hforks
@@ -9966,7 +9985,8 @@ theorem wp_store8Memory64
         { store with wasm :=
             { store.wasm with
               mem := store.wasm.mem.write8 (address.toUInt32 + offset) value.toUInt8 } }⟩ := by
-    simpa only [Wasm.SmallStep.setMemory_eq] using Step.store8Memory64 hbound
+    simpa only [Wasm.SmallStep.setMemory_eq] using
+      Step.store8 (α := α) (address := Value.i64 address) rfl hbound
   obtain ⟨rfl, hconfig⟩ := step_deterministic expectedStep wasmStep
   have parts := Config.mk.inj hconfig
   have hexpr := parts.1
@@ -10030,7 +10050,8 @@ theorem wp_store16Memory64
           { store.wasm with
             mem := store.wasm.mem.write16 (address.toUInt32 + offset) value } },
       [], ⟨rfl, _, rfl,
-        by simpa only [Wasm.SmallStep.setMemory_eq] using Step.store16Memory64 hbound⟩⟩
+        by simpa only [Wasm.SmallStep.setMemory_eq] using
+          Step.store16 (α := α) (address := Value.i64 address) rfl hbound⟩⟩
   iintro !> %e₂ %store₂ %forks %Hstep Hcredit
   rcases Hstep with ⟨hforks, kind, hobs, wasmStep⟩
   change forks = [] at hforks
@@ -10044,7 +10065,8 @@ theorem wp_store16Memory64
         { store with wasm :=
             { store.wasm with
               mem := store.wasm.mem.write16 (address.toUInt32 + offset) value } }⟩ := by
-    simpa only [Wasm.SmallStep.setMemory_eq] using Step.store16Memory64 hbound
+    simpa only [Wasm.SmallStep.setMemory_eq] using
+      Step.store16 (α := α) (address := Value.i64 address) rfl hbound
   obtain ⟨rfl, hconfig⟩ := step_deterministic expectedStep wasmStep
   have parts := Config.mk.inj hconfig
   have hexpr := parts.1
@@ -10108,7 +10130,9 @@ theorem wp_load32Memory64
     exact ⟨[],
       .running ⟨⟨params, localValues, .i32 word :: values⟩,
         code, arity, remainder, controls, calls⟩,
-      store, [], ⟨rfl, _, rfl, by simpa [Hread] using Step.load32Memory64 hbound⟩⟩
+      store, [], ⟨rfl, _, rfl,
+        by simpa [Hread] using
+          Step.load32 (α := α) (address := Value.i64 address) rfl hbound⟩⟩
   iintro !> %e₂ %store₂ %forks %Hstep Hcredit
   rcases Hstep with ⟨hforks, kind, hobs, wasmStep⟩
   change forks = [] at hforks
@@ -10120,7 +10144,8 @@ theorem wp_load32Memory64
       (.instruction (.load32 offset))
       ⟨.running ⟨⟨params, localValues, .i32 word :: values⟩,
         code, arity, remainder, controls, calls⟩, store⟩ := by
-    simpa [Hread] using Step.load32Memory64 hbound
+    simpa [Hread] using
+      Step.load32 (α := α) (address := Value.i64 address) rfl hbound
   obtain ⟨rfl, hconfig⟩ := step_deterministic expectedStep wasmStep
   have parts := Config.mk.inj hconfig
   have hexpr := parts.1
@@ -10183,7 +10208,8 @@ theorem wp_store32Memory64
           { store.wasm with
             mem := store.wasm.mem.write32 (address.toUInt32 + offset) value } },
       [], ⟨rfl, _, rfl,
-        by simpa only [Wasm.SmallStep.setMemory_eq] using Step.store32Memory64 hbound⟩⟩
+        by simpa only [Wasm.SmallStep.setMemory_eq] using
+          Step.store32 (α := α) (address := Value.i64 address) rfl hbound⟩⟩
   iintro !> %e₂ %store₂ %forks %Hstep Hcredit
   rcases Hstep with ⟨hforks, kind, hobs, wasmStep⟩
   change forks = [] at hforks
@@ -10197,7 +10223,8 @@ theorem wp_store32Memory64
         { store with wasm :=
             { store.wasm with
               mem := store.wasm.mem.write32 (address.toUInt32 + offset) value } }⟩ := by
-    simpa only [Wasm.SmallStep.setMemory_eq] using Step.store32Memory64 hbound
+    simpa only [Wasm.SmallStep.setMemory_eq] using
+      Step.store32 (α := α) (address := Value.i64 address) rfl hbound
   obtain ⟨rfl, hconfig⟩ := step_deterministic expectedStep wasmStep
   have parts := Config.mk.inj hconfig
   have hexpr := parts.1
